added constructor, can't figure out why it won't verify

NoC_Modular/FMCAD25/router.dfy
@@ -15,6 +15,7 @@ class Router<T(0,==)> {
   ghost predicate Valid()
     reads this
     reads priority_list
+    reads ids
   {
     // ensures all "channel"-related array lengths are 5, as there are 
     // 5 channels out of the router
@@ -23,10 +24,52 @@ class Router<T(0,==)> {
     && used.Length == 5
     // Ensure every element in the priority list is always unique
     && (forall i: nat, j: nat :: 
-        && i < priority_list.Length 
-        && j < priority_list.Length 
+        && 0 < i < priority_list.Length 
+        && 0 < j < priority_list.Length 
         && i != j 
         && priority_list[i] != priority_list[j])
+    // Ensures all destination id's are unique (or NC)
+    && (forall id1, id2 :: 
+        && id1 in ids[..]
+        && id2 in ids[..]
+        && (id1 != id2 || id1 == NoConnect || id2 == NoConnect))
+  }
+
+  constructor (buffer_capacity: nat, ids: seq<Id>)
+    requires buffer_capacity > 0
+    requires |ids| > 0
+    requires forall id1, id2 :: 
+        && id1 in ids
+        && id2 in ids
+        && (id1 != id2 || id1 == NoConnect || id2 == NoConnect)
+    ensures Valid()
+  {
+    this.ids := new Id[ |ids| ];
+    var default_channel := new Channel<T>(buffer_capacity);
+    this.channels := new Channel<T>[5](_ => default_channel);
+    this.priority_list := new Neighbor[5];
+    this.used := new bool[5](_ => false);
+
+    new; // tbh not sure why I need this
+
+    forall i | 0 <= i < this.ids.Length { this.ids[i] := ids[i]; }
+
+    this.priority_list[0] := North;
+    this.priority_list[1] := East;
+    this.priority_list[2] := South;
+    this.priority_list[3] := West;
+    this.priority_list[4] := Local;
+
+    assert priority_list[0] != priority_list[1];
+    assert priority_list[0] != priority_list[2];
+    assert priority_list[0] != priority_list[3];
+    assert priority_list[0] != priority_list[4];
+    assert priority_list[1] != priority_list[2];
+    assert priority_list[1] != priority_list[3];
+    assert priority_list[1] != priority_list[4];
+    assert priority_list[2] != priority_list[3];
+    assert priority_list[2] != priority_list[4];
+    assert priority_list[3] != priority_list[4];
   }
 
 }
